isabelle/Subst.thy
@@ -2,66 +2,83 @@ theory Subst
   imports Syntax
 begin
 
-fun liftE :: "nat \<Rightarrow> nat \<Rightarrow> exp \<Rightarrow> exp" ("\<up>\<^sub>e")
-and liftV :: "nat \<Rightarrow> nat \<Rightarrow> val \<Rightarrow> val" ("\<up>\<^sub>v")
+text \<open>To bootstrap things, we have to define bind for val, and that requires
+lift for val. Then we can introduce the has_vars class, and from then on
+deal with that only\<close>
+
+fun liftE :: "nat \<Rightarrow> nat \<Rightarrow> exp \<Rightarrow> exp"
+and liftV :: "nat \<Rightarrow> nat \<Rightarrow> val \<Rightarrow> val"
 where
-  "\<up>\<^sub>e n k (Val v) = Val (\<up>\<^sub>v n k v)"
-| "\<up>\<^sub>e n k (Seq e1 e2) = (Seq (\<up>\<^sub>e n k e1) (\<up>\<^sub>e n k e2))"
-| "\<up>\<^sub>e n k (Bar e1 e2) = (Bar (\<up>\<^sub>e n k e1) (\<up>\<^sub>e n k e2))"
-| "\<up>\<^sub>e n k (Uni e1 e2) = (Uni (\<up>\<^sub>e n k e1) (\<up>\<^sub>e n k e2))"
-| "\<up>\<^sub>e n k (App e1 e2) = (App (\<up>\<^sub>v n k e1) (\<up>\<^sub>v n k e2))"
-| "\<up>\<^sub>e n k (Def e) = Def (\<up>\<^sub>e n (k+1) e)"
-| "\<up>\<^sub>e n k (One e) = (One (\<up>\<^sub>e n k e))"
-| "\<up>\<^sub>e n k (All e) = (All (\<up>\<^sub>e n k e))"
-| "\<up>\<^sub>e n k Fail = Fail"
-| "\<up>\<^sub>v n k (Var i) = Var (if i < k then i else i + n)"
-| "\<up>\<^sub>v n k (Const c) = (Const c)"
-| "\<up>\<^sub>v n k (Tup vs) = Tup (map (\<up>\<^sub>v n k) vs)"
-| "\<up>\<^sub>v n k (Lam e) = Lam (\<up>\<^sub>e n (k+1) e)"
-| "\<up>\<^sub>v n k (Op op) = Op op"
+  "liftE n k (Val v) = Val (liftV n k v)"
+| "liftE n k (Seq e1 e2) = (Seq (liftE n k e1) (liftE n k e2))"
+| "liftE n k (Bar e1 e2) = (Bar (liftE n k e1) (liftE n k e2))"
+| "liftE n k (Uni e1 e2) = (Uni (liftE n k e1) (liftE n k e2))"
+| "liftE n k (App v1 v2) = (App (liftV n k v1) (liftV n k v2))"
+| "liftE n k (Def e) = Def (liftE n (k+1) e)"
+| "liftE n k (One e) = (One (liftE n k e))"
+| "liftE n k (All e) = (All (liftE n k e))"
+| "liftE n k Fail = Fail"
+| "liftV n k (Var i) = Var (if i < k then i else i + n)"
+| "liftV n k (Const c) = (Const c)"
+| "liftV n k (Tup vs) = Tup (map (liftV n k) vs)"
+| "liftV n k (Lam e) = Lam (liftE n (k+1) e)"
+| "liftV n k (Op op) = Op op"
 
-lemma liftV_eq_Var[simp]:
-    "(\<up>\<^sub>v n k v = Var i) \<longleftrightarrow> (\<exists> l. (v = Var l \<and> i = (if l < k then l else l + n)))"
-  by (cases v) auto
+lemma liftE1_liftE[simp]:  "l \<le> k \<Longrightarrow> liftE (Suc 0) l (liftE n k e) = liftE n (Suc k) (liftE (Suc 0) l e)"
+and   liftV1_liftV[simp]:  "l \<le> k \<Longrightarrow> liftV (Suc 0) l (liftV n k v) = liftV n (Suc k) (liftV (Suc 0) l v)"
+  by (induction n k e and n k v arbitrary: l and l rule: liftE_liftV.induct) auto
+
+definition lifted :: "nat \<Rightarrow> nat \<Rightarrow> (nat \<Rightarrow> val) \<Rightarrow> (nat \<Rightarrow> val)" where
+  lifted_def_aux: "lifted n k f i =
+      (if     i < k     then liftV n k (f i)
+      else if i < k + n then Var i
+      else                   liftV n k (f (i - n)))"
 
 
-fun delE :: "nat \<Rightarrow> exp \<Rightarrow> exp"
-and delV :: "nat \<Rightarrow> val \<Rightarrow> val"
+lemma lifted_Var[simp]: "lifted n k Var = Var"
+  by (rule; auto simp add: lifted_def_aux)
+
+lemma lifted1_lifted[simp]:
+  "lifted (Suc 0) 0 (lifted n k f) = lifted n (Suc k) (lifted (Suc 0) 0 f)"
+  by (rule; auto simp add: lifted_def_aux)
+
+fun bindE :: "(nat \<Rightarrow> val) \<Rightarrow> exp \<Rightarrow> exp"
+and bindV :: "(nat \<Rightarrow> val) \<Rightarrow> val \<Rightarrow> val"
 where
-  "delE n (Val v) = Val (delV n v)"
-| "delE n(Seq e1 e2) = (Seq (delE n e1) (delE n e2))"
-| "delE n (Bar e1 e2) = (Bar (delE n e1) (delE n e2))"
-| "delE n (Uni e1 e2) = (Uni (delE n e1) (delE n e2))"
-| "delE n (App e1 e2) = (App (delV n e1) (delV n e2))"
-| "delE n (Def e) = Def (delE (Suc n) e)"
-| "delE n (One e) = (One (delE n e))"
-| "delE n (All e) = (All (delE n e))"
-| "delE n Fail = Fail"
-| "delV n (Var i) = Var (if i < n then i else i - 1)"
-| "delV n (Const c) = Const c"
-| "delV n (Tup vs) = Tup (map (delV n) vs)"
-| "delV n (Lam e) = Lam (delE (Suc n) e)"
-| "delV n (Op op) = Op op"
+  "bindE f (Val v1) = Val (bindV f v1)"
+| "bindE f (Seq e1 e2) = Seq (bindE f e1) (bindE f e2)"
+| "bindE f (Bar e1 e2) = Bar (bindE f e1) (bindE f e2)"
+| "bindE f (Uni e1 e2) = Uni (bindE f e1) (bindE f e2)"
+| "bindE f (App v1 v2) = App (bindV f v1) (bindV f v2)"
+| "bindE f (Def e) = Def (bindE (lifted 1 0 f) e)"
+| "bindE f (One e) = One (bindE f e)"
+| "bindE f (All e) = All (bindE f e)"
+| "bindE f Fail = Fail"
+| "bindV f (Var i) = f i"
+| "bindV f (Const k) = Const k"
+| "bindV f (Tup vs) = Tup (map (bindV f) vs)"
+| "bindV f (Lam e) = Lam (bindE (lifted 1 0 f) e)"
+| "bindV f (Op k) = Op k"
 
+lemma liftE_bindE[simp]: "liftE n k (bindE f e) = bindE (lifted n k f) (liftE n k e)"
+  and liftV_bindV[simp]: "liftV n k (bindV f v) = bindV (lifted n k f) (liftV n k v)"
+by (induction f e and f v arbitrary: k and k rule: bindE_bindV.induct) (auto simp add: lifted_def_aux)
 
-fun substE :: "nat \<Rightarrow> val \<Rightarrow> exp \<Rightarrow> exp"
-and substV :: "nat \<Rightarrow> val \<Rightarrow> val \<Rightarrow> val"
-where
-  "substE n v (Val v1) = Val (substV n v v1)"
-| "substE n v (Seq e1 e2) = Seq (substE n v e1) (substE n v e2)"
-| "substE n v (Bar e1 e2) = Bar (substE n v e1) (substE n v e2)"
-| "substE n v (Uni e1 e2) = Uni (substE n v e1) (substE n v e2)"
-| "substE n v (App v1 v2) = App (substV n v v1) (substV n v v2)"
-| "substE n v (Def e) = Def (substE (n+1) (\<up>\<^sub>v 1 0 v) e)"
-| "substE n v (One e) = One (substE n v e)"
-| "substE n v (All e) = All (substE n v e)"
-| "substE n v Fail = Fail"
-| "substV n v (Var i) = (if i = n then v else Var i)"
-| "substV n v (Const k) = Const k"
-| "substV n v (Tup vs) = Tup (map (substV n v) vs)"
-| "substV n v (Lam e) = Lam (substE (n+1) (\<up>\<^sub>v 1 0 v) e)"
-| "substV n v (Op k) = Op k"
+lemma  lifted_bindV[simp]: "lifted n k (\<lambda>i. bindV f (g i)) = (\<lambda>i. bindV (lifted n k f) (lifted n k g i))"
+  by (auto simp add: lifted_def_aux)
 
+lemma bindE_bindE: "bindE f (bindE g e) = bindE (\<lambda> n. bindV f (g n)) e"
+and bindV_bindV:   "bindV f (bindV g v) = bindV (\<lambda> n. bindV f (g n)) v"
+  by (induction g e and g v arbitrary: f and f rule: bindE_bindV.induct) auto
+
+lemma bindE_Var: "bindE Var e = e"
+and bindV_Var:   "bindV Var v = v"
+  by (induction e and v) (auto simp add: map_idI)
+
+lemma liftE_is_bindE: "liftE n k e = bindE (\<lambda>i. Var (if i < k then i else i + n)) e"
+and liftV_is_bindV: "liftV n k v = bindV (\<lambda>i. Var (if i < k then i else i + n)) v"
+  by (induction n k e and n k v rule: liftE_liftV.induct)
+     (auto 4 4 simp add: lifted_def_aux intro!: arg_cong2[where f= bindE])
 
 fun occursE :: "nat \<Rightarrow> exp \<Rightarrow> bool"
 and occursV :: "nat \<Rightarrow> val \<Rightarrow> bool"
@@ -81,35 +98,185 @@ where
 | "occursV n (Lam e) \<longleftrightarrow> occursE (n+1) e"
 | "occursV n (Op op) \<longleftrightarrow> False"
 
-
-lemma occursE_bars[simp]:
-  "occursE n (bars es) \<longleftrightarrow> (\<exists> e \<in> set es. occursE n e)"
-by (induction es rule: bars.induct) auto
-
-lemma occursE_seqs[simp]:
-  "occursE n (seqs es) \<longleftrightarrow> (\<exists> e \<in> set es. occursE n e)"
-by (induction es rule: seqs.induct) auto
-
-lemma occursE_liftE: "occursE n (\<up>\<^sub>e k j e) \<longleftrightarrow>
+lemma occursE_liftE: "occursE n (liftE k j e) \<longleftrightarrow>
     (if n < j then occursE n e else if n < j + k then False else  occursE (n - k) e)"
-  and occursV_liftV: "occursV n (\<up>\<^sub>v k j v) \<longleftrightarrow>
+  and occursV_liftV: "occursV n (liftV k j v) \<longleftrightarrow>
     (if n < j then occursV n v else if n < j + k then False else  occursV (n - k) v)"
   by (induction k j e and k j v arbitrary: n and n rule: liftE_liftV.induct)
      (auto simp add: Suc_diff_le)
 
-lemma occursE_delE[simp]: "\<not> occursE n e \<Longrightarrow>
-  occursE k (delE n e) = (if k < n then occursE k e else occursE (Suc k) e)"
-and occursV_delV[simp]: "\<not> occursV n v \<Longrightarrow>
-  occursV k (delV n v) = (if k < n then occursV k v else occursV (Suc k) v)"
-  by (induction n e and n v arbitrary: k and k rule: delE_delV.induct) auto
+lemma occursE_bindE: "occursE i (bindE f e) \<longleftrightarrow> (\<exists> n. occursE n e \<and> occursV i (f n))"
+and   occursV_bindV: "occursV i (bindV f v) \<longleftrightarrow> (\<exists> n. occursV n v \<and> occursV i (f n))"
+  apply (induction f e and f v arbitrary: i and i rule: bindE_bindV.induct)
+               apply (auto simp add: occursV_liftV simp add: lifted_def_aux)
+   apply force
+  apply force
+  done
 
-lemma occursE_substE[simp]:
-  "occursE i (substE n v e) \<longleftrightarrow> 
-  (i \<noteq> n \<and> occursE i e) \<or> (occursE n e \<and> occursV i v)"
-and occursV_substV[simp]:
-  "occursV i (substV n v v') \<longleftrightarrow> 
-  (i \<noteq> n \<and> occursV i v') \<or> (occursV n v' \<and> occursV i v)"
-  by (induction n v e and n v v' arbitrary: i and i rule: substE_substV.induct)
-     (auto simp add: occursV_liftV)
-  
+lemma liftV_eq_iff[simp]:
+  "liftV n k v = Var i \<longleftrightarrow> (i < k \<and> v = Var i) \<or> (i \<ge> k + n \<and> v = Var (i - n))"
+  by (cases v) auto 
+
+lemma lifted_eq_var_iff[simp]:
+  "lifted n k f i = Var i \<longleftrightarrow> (i < k \<and> f i = Var i) \<or> (i \<ge> k \<and> i < k + n) \<or> (i \<ge> k + n \<and> f (i - n) = Var (i - n))"
+  by (auto simp add: lifted_def_aux)
+
+lemma map_idE[elim_format, elim]:
+  "map f xs = xs \<Longrightarrow> x \<in> set xs \<Longrightarrow> f x = x"
+  using map_eq_conv by fastforce
+
+lemma bindE_id_iff:
+  "bindE f e = e \<longleftrightarrow> (\<forall> n. occursE n e \<longrightarrow> f n = Var n)" 
+and  bindV_id_iff:
+  "bindV f v = v \<longleftrightarrow> (\<forall> n. occursV n v \<longrightarrow> f n = Var n)"
+  by (induction f e and f v  rule: bindE_bindV.induct)
+     (auto intro!:  map_idI elim!: map_idE[OF sym])
+
+
+text \<open>Now we can define the has_vars class (we cannot do it earlier because we need bind for var)\<close>
+
+class has_vars =
+  fixes bind :: "(nat \<Rightarrow> val) \<Rightarrow> 'a \<Rightarrow> 'a"
+  fixes occurs :: "nat \<Rightarrow> 'a \<Rightarrow> bool"
+  assumes bind_bind_aux: "bind f (bind g x) = bind (\<lambda> n. bindV f (g n)) x"
+  assumes occurs_bind_aux: "occurs i (bind f x) \<longleftrightarrow> (\<exists> n. occurs n x \<and> occursV i (f n))"
+  assumes bind_id_iff: "bind f x = x \<longleftrightarrow> (\<forall> n. occurs n x \<longrightarrow> f n = Var n)"
+
+
+text \<open>The instance for exp and val uses the definitions and lemmas above.\<close>
+
+instantiation exp :: has_vars begin
+  definition "bind = bindE"
+  definition "occurs = occursE"
+  instance
+    by (standard; simp only: bind_exp_def occurs_exp_def
+        bindE_bindE bindE_Var occursE_bindE bindE_id_iff)
+end
+
+instantiation val :: has_vars begin
+  definition "bind = bindV"
+  definition "occurs = occursV"
+  instance
+    by (standard; simp add: bind_val_def occurs_val_def
+        bindV_bindV bindV_Var occursV_bindV bindV_id_iff)
+end
+
+text \<open>Substitution and renumbering is now derived from bind\<close>
+
+definition renumber :: "(nat \<Rightarrow> nat) \<Rightarrow> 'a::has_vars \<Rightarrow> 'a" where
+  "renumber f = bind (\<lambda> i. Var (f i))"
+
+definition bumpAt :: "nat \<Rightarrow> nat \<Rightarrow> (nat \<Rightarrow> nat)" where
+  "bumpAt n k i = (if i < k then i else i + n)"
+
+definition liftedN :: "nat \<Rightarrow> nat \<Rightarrow> (nat \<Rightarrow> nat) \<Rightarrow> (nat \<Rightarrow> nat)" where
+  "liftedN n k f i =
+      (if     i < k     then bumpAt n k (f i)
+      else if i < k + n then i
+      else                   bumpAt n k (f (i - n)))"
+
+
+abbreviation lift :: "'a::has_vars \<Rightarrow> 'a" ("\<up>") where
+  "\<up> \<equiv> renumber Suc"
+
+definition delN :: "nat \<Rightarrow> (nat \<Rightarrow> nat)" where
+  "delN n i = (if i < n then i else i - 1)"
+abbreviation del :: "nat \<Rightarrow> 'a::has_vars \<Rightarrow> 'a" where
+  "del n \<equiv> renumber (delN n)"
+abbreviation subst :: "nat \<Rightarrow> val \<Rightarrow> 'a::has_vars \<Rightarrow> 'a" where
+  "subst n v \<equiv> bind (Var(n := v))"
+
+
+text \<open>From now on we want to only use the overloaded variants for exp and var\<close>
+
+lemmas bind_exp_simps[simp] = bindE.simps[folded bind_exp_def bind_val_def]
+lemmas bind_val_simps[simp] = bindV.simps[folded bind_exp_def bind_val_def]
+lemmas occurs_exp_simps[simp] = occursE.simps[folded occurs_exp_def occurs_val_def]
+lemmas occurs_val_simps[simp] = occursV.simps[folded occurs_exp_def occurs_val_def]
+lemmas bind_bind = bind_bind_aux[folded bind_val_def]
+lemmas occurs_bind = occurs_bind_aux[folded occurs_val_def]
+
+lemma liftV_eq_renumber: "liftV n k = renumber (bumpAt n k)"
+  unfolding liftV_is_bindV renumber_def bind_val_def bumpAt_def
+  by rule rule
+
+lemmas lifted_def = lifted_def_aux[unfolded liftV_eq_renumber]
+
+
+lemma has_varsI[case_names Bind_bind Occurs_bind Bind_id_iff]:
+  fixes bind' occurs'
+  assumes "\<And> f g x. bind' f (bind' g x) = bind' (\<lambda> n. bind f (g n)) x"
+  assumes "\<And> i f e. occurs' i (bind' f e) \<longleftrightarrow> (\<exists> n. occurs' n e \<and> occurs i (f n))"
+  assumes "\<And> f e. bind' f e = e \<longleftrightarrow> (\<forall>n. occurs' n e \<longrightarrow> f n = Var n)"
+  shows "class.has_vars bind' occurs'"
+  by (rule class.has_vars.intro) (intro assms[unfolded bind_val_def occurs_val_def])+
+
+hide_const liftE bindE occursE
+hide_const liftV bindV occursV
+
+text \<open>Additional lemmas for exp and val\<close>
+
+lemma bind_lifted_Var_f:
+  "bind (lifted k l (\<lambda>n. Var (f n))) = renumber (liftedN k l f)"
+  unfolding renumber_def lifted_def liftedN_def
+  by (rule arg_cong[where f = bind]) auto
+
+(* Make sure no bind remains *)
+lemmas renumber_exp_simps[simp] =
+  bind_exp_simps[where f = "\<lambda> n. Var (f n)" for f, folded renumber_def, unfolded bind_lifted_Var_f]
+lemmas renumber_val_simps[simp] =
+  bind_val_simps[where f = "\<lambda> n. Var (f n)" for f, folded renumber_def, unfolded bind_lifted_Var_f]
+
+(*
+lemma liftV_eq_Var[simp]:
+    "(lift n k v = Var i) \<longleftrightarrow> (\<exists> l. (v = Var l \<and> i = (if l < k then l else l + n)))"
+  by (cases v) auto
+*)
+
+lemma occurs_bars[simp]:
+  "occurs n (bars es) \<longleftrightarrow> (\<exists> e \<in> set es. occurs n e)"
+by (induction es rule: bars.induct) auto
+
+lemma occurs_seqs[simp]:
+  "occurs n (seqs es) \<longleftrightarrow> (\<exists> e \<in> set es. occurs n e)"
+by (induction es rule: seqs.induct) auto
+
+text "Derived lemmas"
+
+lemma bind_id_iff2: "x = bind f x \<longleftrightarrow> (\<forall> n. occurs n x \<longrightarrow> f n = Var n)"
+  by (metis bind_id_iff)
+
+lemma bind_Var[simp]: "bind Var x = x"
+  by (simp add: bind_id_iff)
+
+lemma renumber_id[simp]: "renumber id x = x"
+  unfolding renumber_def by simp
+
+lemma bumpAt_0[simp]: "bumpAt 0 k = id"
+  by rule (auto simp add: bumpAt_def)
+
+lemma lifted_0[simp]: "lifted 0 k f = f"
+  by (rule; auto simp add: lifted_def)
+ 
+lemma occurs_renumber:
+  "occurs n (renumber f e) = (\<exists> i. occurs i e \<and> n = f i)"
+  unfolding renumber_def by (auto simp add: occurs_bind)
+
+lemma occurs_del[simp]: "\<not> occurs n e \<Longrightarrow>
+  occurs k (del n e) = (if k < n then occurs k e else occurs (Suc k) e)"
+  unfolding delN_def occurs_renumber
+  by (smt (verit, ccfv_SIG) diff_Suc_1 less_Suc_eq_0_disj less_imp_diff_less linorder_neqE_nat not_less_eq)
+
+lemma occurs_lift[simp]: "occurs n (\<up> x) = (n > 0 \<and> occurs (n - 1) x)"
+  unfolding  occurs_renumber by auto
+
+
+lemma occurs_subst[simp]:
+  "occurs i (subst n v e) \<longleftrightarrow> (i \<noteq> n \<and> occurs i e) \<or> (occurs n e \<and> occurs i v)"
+ by (auto simp add: occurs_bind)
+
+lemma lifted_bind[simp]: "lifted n k (\<lambda>i. bind f (g i)) = (\<lambda>i. bind (lifted n k f) (lifted n k g i))"
+  by rule (auto intro!: arg_cong2[where f = bind] simp add: lifted_def renumber_def bind_bind bumpAt_def)
+
+
 end
