isabelle/SubstContext.thy
@@ -2,206 +2,166 @@ theory SubstContext
 imports Subst Contexts
 begin
 
-fun (sequential) depthECE :: "ece \<Rightarrow> nat" where
-  "depthECE (CVal _) = 1"
-| "depthECE CDef = 1"
-| "depthECE (CAppl _ _) = 1"
-| "depthECE (CAppr _ _) = 1"
-| "depthECE _ = 0"
+class has_depth = has_vars +
+  fixes depth :: "'a \<Rightarrow> nat"
+  assumes depth_bind[simp]: "depth (bind f x) = depth x"
 
-definition depthEC :: "ec \<Rightarrow> nat" where
-  "depthEC ec = sum_list (map depthECE ec)"
+lemma depth_del[simp]: "depth (renumber f x) = depth x"
+  unfolding renumber_def by simp
 
-lemma depthECE_isXE[simp]: "isXE ece \<Longrightarrow> depthECE ece = 0"
-  by (induction ece) (auto elim: isXE.cases)
+instantiation list :: (has_depth) has_vars 
+begin
 
-lemma depthEC_isX[simp]: "isX ec \<Longrightarrow> depthEC ec = 0"
-  by (induction ec) (auto simp add: isX_def depthEC_def)
+fun bind_list where
+  "bind_list f [] = []"
+| "bind_list f (x # xs) = bind f x # bind_list (lifted (depth x) 0 f) xs"
 
-lemma depthEC_replicate[simp]: "depthEC (replicate n ece) = n * depthECE ece"
-  by (auto simp add: depthEC_def sum_list_replicate)
+fun occurs_list where
+  "occurs_list n [] = False"
+| "occurs_list n (x # xs) \<longleftrightarrow> occurs n x \<or> occurs_list (depth x + n) xs"
 
+instance
+proof (rule Subst.has_vars_class.intro, (intro_classes)[1], induction rule: has_varsI)
+  case (Bind_bind f g xs)
+  show ?case
+    by (induction g xs arbitrary: f rule:bind_list.induct) (auto simp add: bind_bind)
+next
+  case (Occurs_bind i f xs)
+  show ?case
+    apply (induction f xs arbitrary: i rule:bind_list.induct)
+     apply (auto simp add: occurs_bind lifted_def renumber_def bumpAt_def)
+    apply (metis add_diff_inverse_nat)
+    done
+next
+  case (Bind_id_iff f xs)
+  show ?case
+    by (induction f xs rule:bind_list.induct) (auto simp add: bind_id_iff)
+qed
+end
+                                     
+instantiation list :: (has_depth) has_depth
+begin
+definition depth_list :: "'a list \<Rightarrow> nat" where
+  "depth_list xs = sum_list (map depth xs)"
+instance
+proof
+  fix f and xs :: "'a list"
+  show "depth (bind f xs) = depth xs"
+    by (induction xs arbitrary: f) (auto simp add: depth_list_def)
+qed
+end
 
-fun liftVCE :: "nat \<Rightarrow> nat \<Rightarrow> vce \<Rightarrow> vce" where
-  "liftVCE n k (CTup vs1 vs2) = CTup (map (liftV n k) vs1) (map (liftV n k) vs2)"
+lemmas renumber_list_simps[simp] =
+  bind_list.simps[where f = "\<lambda> n. Var (f n)" for f, folded renumber_def, unfolded bind_lifted_Var_f]
 
-definition liftVC :: "nat \<Rightarrow> nat \<Rightarrow> vc \<Rightarrow> vc" where
-  "liftVC n k vc = map (liftVCE n k) vc"
-
-fun liftECE :: "nat \<Rightarrow> nat \<Rightarrow> ece \<Rightarrow> ece" where
-  "liftECE n k (CVal vc) = CVal (liftVC n k vc)"
-| "liftECE n k CDef = CDef"
-| "liftECE n k (CAppl vc v2) = CAppl (liftVC n k vc) (liftV n k v2)"
-| "liftECE n k (CAppr v1 vc) = CAppr (liftV n k v1) (liftVC n k vc)"
-| "liftECE n k (CSeql e2) = CSeql (liftE n k e2)"
-| "liftECE n k (CSeqr e1) = CSeqr (liftE n k e1)"
-| "liftECE n k (CBarl e2) = CBarl (liftE n k e2)"
-| "liftECE n k (CBarr e1) = CBarr (liftE n k e1)"
-| "liftECE n k (CUnil e2) = CUnil (liftE n k e2)"
-| "liftECE n k (CUnir e1) = CUnir (liftE n k e1)"
-| "liftECE n k COne = COne"
-| "liftECE n k CAll = CAll"
-
-fun liftEC :: "nat \<Rightarrow> nat \<Rightarrow> ec \<Rightarrow> ec" where
-  "liftEC n k [] = []" 
-| "liftEC n k (ece#ec) = liftECE n k ece # liftEC n (depthECE ece + k) ec" 
-
-lemma depthECE_liftECE[simp]: "depthECE (liftECE n k ece) = depthECE ece"
-  by (cases ece) auto
-
-lemma depthEC_liftEC [simp]: "depthEC (liftEC n k ec) = depthEC ec"
-  by (induction n k ec rule: liftEC.induct) (auto simp add: depthEC_def)
-
-fun delVCE :: "nat \<Rightarrow> vce \<Rightarrow> vce" where
-  "delVCE n (CTup vs1 vs2) = CTup (map (delV n) vs1) (map (delV n) vs2)"
-
-definition delVC :: "nat \<Rightarrow> vc \<Rightarrow> vc" where
-  "delVC n vc = map (delVCE n) vc"
-
-fun delECE :: "nat \<Rightarrow> ece \<Rightarrow> ece" where
-  "delECE n (CVal vc) = CVal (delVC n vc)"
-| "delECE n CDef = CDef"
-| "delECE n (CAppl vc v2) = CAppl (delVC n vc) (delV n v2)"
-| "delECE n (CAppr v1 vc) = CAppr (delV n v1) (delVC n vc)"
-| "delECE n (CSeql e2) = CSeql (delE n e2)"
-| "delECE n (CSeqr e1) = CSeqr (delE n e1)"
-| "delECE n (CBarl e2) = CBarl (delE n e2)"
-| "delECE n (CBarr e1) = CBarr (delE n e1)"
-| "delECE n (CUnil e2) = CUnil (delE n e2)"
-| "delECE n (CUnir e1) = CUnir (delE n e1)"
-| "delECE n COne = COne"
-| "delECE n CAll = CAll"
-
-fun delEC :: "nat \<Rightarrow> ec \<Rightarrow> ec" where
-  "delEC n [] = []" 
-| "delEC n (ece#ec) = delECE n ece # delEC (depthECE ece + n) ec" 
+lemma depth_replicate[simp]: "depth (replicate n xs) = n * depth xs"
+  by (auto simp add: depth_list_def sum_list_replicate)
 
 
-lemma depthECE_delECE[simp]: "depthECE (delECE n ece) = depthECE ece"
-  by (induction ece) auto
+instantiation vce :: has_vars 
+begin
+fun bind_vce :: "(nat \<Rightarrow> val) \<Rightarrow> vce \<Rightarrow> vce" where
+  "bind_vce f (CTup vs1 vs2) = CTup (map (bind f) vs1) (map (bind f) vs2)"
 
-lemma depthEC_delEC[simp]: "depthEC (delEC n ec) = depthEC ec"
-  by (induction n ec rule: delEC.induct) (auto simp add: depthEC_def)
+fun occurs_vce :: "nat \<Rightarrow> vce \<Rightarrow> bool" where
+  "occurs_vce n (CTup vs1 vs2) \<longleftrightarrow> (\<exists> v \<in> set vs1. occurs n v) \<or> (\<exists> v \<in> set vs2. occurs n v)"
 
+instance
+proof (rule Subst.has_vars_class.intro, (intro_classes)[1], induction rule: has_varsI)
+  case (Bind_bind f g x)
+  show ?case by (cases x)(simp add: bind_bind)
+next
+  case (Occurs_bind i f x)
+  show ?case by (cases x)(auto simp add: occurs_bind)
+next
+  case (Bind_id_iff f x)
+  show ?case by (cases x)(auto 4 4 simp add: bind_id_iff intro!: map_idI)
+qed
+end
 
-fun substVCE :: "nat \<Rightarrow> val \<Rightarrow> vce \<Rightarrow> vce" where
-  "substVCE n v (CTup vs1 vs2) = CTup (map (substV n v) vs1) (map (substV n v) vs2)"
+lemmas renumber_vce_simps[simp] = bind_vce.simps[where f = "\<lambda> n. Var (f n)" for f, folded renumber_def]
 
-definition substVC :: "nat \<Rightarrow> val \<Rightarrow> vc \<Rightarrow> vc" where
-  "substVC n v vc = map (substVCE n v) vc"
-
-fun substECE :: "nat \<Rightarrow> val \<Rightarrow> ece \<Rightarrow> ece" where
-  "substECE n v (CVal vc) = CVal (substVC n v vc)"
-| "substECE n v CDef = CDef"
-| "substECE n v (CAppl vc v2) = CAppl (substVC n v vc) (substV n v v2)"
-| "substECE n v (CAppr v1 vc) = CAppr (substV n v v1) (substVC n v vc)"
-| "substECE n v (CSeql e2) = CSeql (substE n v e2)"
-| "substECE n v (CSeqr e1) = CSeqr (substE n v e1)"
-| "substECE n v (CBarl e2) = CBarl (substE n v e2)"
-| "substECE n v (CBarr e1) = CBarr (substE n v e1)"
-| "substECE n v (CUnil e2) = CUnil (substE n v e2)"
-| "substECE n v (CUnir e1) = CUnir (substE n v e1)"
-| "substECE n v COne = COne"
-| "substECE n v CAll = CAll"
-
-fun substEC :: "nat \<Rightarrow> val \<Rightarrow> ec \<Rightarrow> ec" where
-  "substEC n v [] = []" 
-| "substEC n v (ece#ec) = substECE n v ece # substEC (depthECE ece + n) (\<up>\<^sub>v (depthECE ece) 0 v) ec" 
-
-lemma depthECE_substECE[simp]: "depthECE (substECE n v ece) = depthECE ece"
-  by (induction ece) auto
-
-lemma depthEC_substEC[simp]: "depthEC (substEC n v ec) = depthEC ec"
-  by (induction ec arbitrary: n v) (auto simp add: depthEC_def)
-
-fun occursVCE where
-  "occursVCE n (CTup vs1 vs2) \<longleftrightarrow> (\<exists> v \<in> set vs1. occursV n v) \<or>  (\<exists> v \<in> set vs2. occursV n v)"
-
-definition occursVC where "occursVC n vc \<longleftrightarrow> (\<exists> vce \<in> set vc. occursVCE n vce)"
-
-lemma occursVC_Nil[simp]: "occursVC n [] = False"
-  by (simp add: occursVC_def appVC_def appVC'_def)
-
-lemma occursVC_Cons[simp]: "occursVC n (vce # vc) = occursVCE n vce \<or> occursVC n vc"
-  by (auto simp add: occursVC_def appVC_def appVC'_def)
-
-definition "occursECE n ece = occursE n (appECE ece Fail)"
-
-fun occursEC where
-  "occursEC n [] = False"
-| "occursEC n (ece # ec) \<longleftrightarrow> occursECE n ece \<or> occursEC (depthECE ece + n) ec"
-
-
-lemma occursV_appVCE[simp]:
-  "occursV n (appVCE vce v) \<longleftrightarrow> occursV n v \<or> occursVCE n vce"
+lemma occurs_appVCE[simp]:
+  "occurs n (appVCE vce v) \<longleftrightarrow> occurs n v \<or> occurs n vce"
   by (cases vce) auto
 
-lemma occursE_appVC[simp]:
-  "occursV n (appVC vc e) \<longleftrightarrow> occursE (1 + n) e \<or> occursVC n vc"
-  by (induction vc) (auto simp add: appVC_def appVC'_def occursVC_def)
+instantiation vce :: has_depth
+begin
+fun depth_vce :: "vce \<Rightarrow> nat" where "depth_vce vce = 0"
+instance by standard simp
+end
 
-lemma occursE_appECE[simp]:
-  "occursE n (appECE ece e) \<longleftrightarrow> occursE (depthECE ece + n) e \<or> occursECE n ece"
-  by (cases ece) (auto simp add: occursECE_def)
+lemma occurs_appVC[simp]:
+  "occurs n (appVC vc e) \<longleftrightarrow> occurs (1 + n) e \<or> occurs n vc"
+  by (induction vc) (auto simp add: appVC_def appVC'_def )
+
+instantiation ece :: has_vars
+begin
+fun bind_ece :: "(nat \<Rightarrow> val) \<Rightarrow> ece \<Rightarrow> ece" where
+  "bind_ece f (CVal vc) = CVal (bind f vc)"
+| "bind_ece f CDef = CDef"
+| "bind_ece f (CAppl vc v2) = CAppl (bind f vc) (bind f v2)"
+| "bind_ece f (CAppr v1 vc) = CAppr (bind f v1) (bind f vc)"
+| "bind_ece f (CSeql e2) = CSeql (bind f e2)"
+| "bind_ece f (CSeqr e1) = CSeqr (bind f e1)"
+| "bind_ece f (CBarl e2) = CBarl (bind f e2)"
+| "bind_ece f (CBarr e1) = CBarr (bind f e1)"
+| "bind_ece f (CUnil e2) = CUnil (bind f e2)"
+| "bind_ece f (CUnir e1) = CUnir (bind f e1)"
+| "bind_ece f COne = COne"
+| "bind_ece f CAll = CAll"
+
+definition "occurs_ece n ece = occurs n (appECE ece Fail)"
+
+instance
+proof (rule Subst.has_vars_class.intro, (intro_classes)[1], induction rule: has_varsI)
+  case (Bind_bind f g ece)
+  show ?case
+    by (cases ece) (auto simp add: bind_bind)
+next
+  case (Occurs_bind i f ece)
+  show ?case
+    by (cases ece) (auto simp add: occurs_bind occurs_ece_def)
+next
+  case (Bind_id_iff f ece)
+  show ?case by (cases ece) (auto simp add: occurs_ece_def bind_id_iff)
+qed
+end
+
+instantiation ece :: has_depth
+begin
+fun (sequential) depth_ece :: "ece \<Rightarrow> nat" where
+  "depth_ece (CVal _) = 1"
+| "depth_ece CDef = 1"
+| "depth_ece (CAppl _ _) = 1"
+| "depth_ece (CAppr _ _) = 1"
+| "depth_ece _ = 0"
+instance
+proof
+  fix f and ece :: ece
+  show "depth (bind f ece) = depth ece"
+    by (cases ece) auto
+qed
+end
+
+lemmas renumber_ece_simps[simp] = bind_ece.simps[where f = "\<lambda> n. Var (f n)" for f, folded renumber_def]
+
+lemma depth_isXE[simp]: "isXE ece \<Longrightarrow> depth ece = 0"
+  by (induction ece) (auto elim: isXE.cases)
+
+lemma depth_isX[simp]: "isX ec \<Longrightarrow> depth ec = 0"
+  by (induction ec) (auto simp add: isX_def depth_list_def)
+
+lemma occurs_appECE[simp]:
+  "occurs n (appECE ece e) \<longleftrightarrow> occurs n ece \<or> occurs (depth ece + n) e"
+  by (cases ece) (auto simp add: occurs_ece_def)
 
 lemma occursE_appEC[simp]:
-  "occursE n (appEC ec e) \<longleftrightarrow> occursE (depthEC ec + n) e \<or> occursEC n ec "
-  apply (induction n ec rule: occursEC.induct)
-   apply (auto simp add: appEC_def depthEC_def)
+  "occurs n (appEC ec e) \<longleftrightarrow> occurs n ec \<or> occurs (depth ec + n) e"
+  apply (induction n ec rule: occurs_list.induct)
+   apply (auto simp add: appEC_def depth_list_def)
   apply (metis ab_semigroup_add_class.add_ac(1) group_cancel.add2)
   apply (simp add: ab_semigroup_add_class.add_ac(1) add.commute)
   done
-
-lemma occursVCE_liftVCE[simp]: "occursVCE n (liftVCE k j vce) \<longleftrightarrow>
-    (if n < j then occursVCE n vce else if n < j + k then False else occursVCE (n - k) vce)"
-  by (cases vce) (auto simp add: occursV_liftV)
-
-lemma occursVC_liftVC[simp]: "occursVC n (liftVC k j vc) \<longleftrightarrow>
-    (if n < j then occursVC n vc else if n < j + k then False else occursVC (n - k) vc)"
-  by (auto simp add: occursVC_def liftVC_def)
-
-lemma occursECE_liftECE[simp]: "occursECE n (liftECE k j ece) \<longleftrightarrow>
-    (if n < j then occursECE n ece else if n < j + k then False else occursECE (n - k) ece)"
-  by (cases ece) (auto simp add: occursECE_def occursV_liftV occursE_liftE)
-
-lemma occursEC_liftEC[simp]: "occursEC n (liftEC k j ec) \<longleftrightarrow>
-    (if n < j then occursEC n ec else if n < j + k then False else occursEC (n - k) ec)"
- by (induction k j ec arbitrary: n rule: liftEC.induct) auto
-
-lemma occursVCE_delEC[simp]: "\<not> occursVCE n vce \<Longrightarrow>
-  occursVCE k (delVCE n vce) = (if k < n then occursVCE k vce else occursVCE (Suc k) vce)"
-  by (cases vce) auto
-
-lemma occursVC_delVC[simp]: "\<not> occursVC n vc \<Longrightarrow>
-  occursVC k (delVC n vc) = (if k < n then occursVC k vc else occursVC (Suc k) vc)"
- by (auto simp add: occursVC_def delVC_def)
-
-lemma occursECE_delEC[simp]: "\<not> occursECE n ece \<Longrightarrow>
-  occursECE k (delECE n ece) = (if k < n then occursECE k ece else occursECE (Suc k) ece)"
- by (cases ece) (auto simp add: occursECE_def)
-
-lemma occursEC_delEC[simp]: "\<not> occursEC n ec \<Longrightarrow>
-  occursEC k (delEC n ec) = (if k < n then occursEC k ec else occursEC (Suc k) ec)"
- by (induction n ec arbitrary: k rule: delEC.induct) auto
-
-lemma occursVCE_substVCE[simp]:
-  "occursVCE i (substVCE n v vce) \<longleftrightarrow> 
-  (i \<noteq> n \<and> occursVCE i vce) \<or> (occursVCE n vce \<and> occursV i v)"
-by (cases vce) auto
-
-lemma occursVC_substVC[simp]:
-  "occursVC i (substVC n v vc) \<longleftrightarrow> 
-  (i \<noteq> n \<and> occursVC i vc) \<or> (occursVC n vc \<and> occursV i v)"
-  by (auto simp add: substVC_def occursVC_def)
-
-lemma occursECE_substECE[simp]:
-  "occursECE i (substECE n v ece) \<longleftrightarrow> 
-  (i \<noteq> n \<and> occursECE i ece) \<or> (occursECE n ece \<and> occursV i v)"
-  by (cases ece) (auto simp add: occursECE_def)
-
-lemma occursEC_substEC[simp]:
-  "occursEC i (substEC n v ec) \<longleftrightarrow> 
-  (i \<noteq> n \<and> occursEC i ec) \<or> (occursEC n ec \<and> occursV i v)"
-  by (induction ec arbitrary: i n v) (auto simp add: occursV_liftV)
 
 end
