isabelle/SubstRecConfluence.thy
@@ -29,31 +29,28 @@ lemma subVC_swap:
   shows    "appVC (subVC vc1 vc2 e2) e1 = appVC (subVC vc2 vc1 e1) e2"
   sorry
 
-lemma liftVC_subVC:
-  "liftVC n k (subVC vc1 vc2 e) = subVC (liftVC n k vc1) (liftVC n k vc2) (liftE n (Suc k) e)"
+lemma renumber_subVC:
+  "renumber f (subVC vc1 vc2 e) = subVC (renumber f vc1) (renumber f vc2) (renumber (liftedN 1 0 f) e)"
   sorry
 
-lemma substVC_subVC:
-  "substVC n v (subVC vc1 vc2 e) = subVC (substVC n v vc1) (substVC n v vc2) (substE (Suc n) (liftV 1 0 v) e)"
+lemma renumber_appVC[simp]: "renumber f (appVC vc e) = appVC (renumber f vc) (renumber (liftedN 1 0 f) e)"
   sorry
 
-lemma liftV_appVC[simp]: "liftV n k (appVC vc e) = appVC (liftVC n k vc) (liftE n (Suc k) e)"
-  sorry
-
-lemma substV_appVC[simp]: "substV n v (appVC vc e) = appVC (substVC n v vc) (substE (Suc n) (liftV 1 0 v) e)"
-  sorry
+(*
 
 lemma liftVC_substVC:
   "liftVC k j (substVC n v vc) =
     (if n < j then substVC n (liftV k j v) (liftVC k j vc)
     else substVC (n+k) (liftV k j v) (liftVC k j vc))"
   sorry
+*)
 
 lemma substVC_dead:
-  "\<not> occursVC n vc \<Longrightarrow> substVC n v vc = vc"
+  "\<not> occurs n vc \<Longrightarrow> subst n v vc = vc"
   sorry
 
 
+(*
 lemma liftVC_liftVC[simp]:
   "l \<le> k2 \<Longrightarrow> k2 \<le> j+l \<Longrightarrow> liftVC k k2 (liftVC j l vc) = liftVC (k+j) l vc"
   sorry
@@ -100,10 +97,20 @@ lemma substE_substE:
   "\<not> occursV n2 v1 \<Longrightarrow>
   substE n1 v1 (substE n2 v2 e) = substE n2 (substV n1 v1 v2) (substE n1 v1 e)"
   sorry
+*)
+
 
 lemma arg_cong3: "\<lbrakk>a = b; c = d; e = g\<rbrakk> \<Longrightarrow> f a c e = f b d g"
   by (iprover intro: refl elim: subst)
 
+lemma renumber_renumber: "renumber f (renumber g x) = renumber (f o g) x"
+  unfolding renumber_def
+  by (auto simp add: renumber_def bind_bind)
+
+lemma [simp]: "n - Suc 0 = 0 \<longleftrightarrow> n = 0 \<or> n = 1" by auto
+
+lemma lifted_simps[simp]: "0 < k \<Longrightarrow> liftedN k n f n = n"
+  unfolding liftedN_def by auto
 
 lemma Subst_Rec_Subst_Rec: "rule_SubstRec\<inverse>\<inverse> OO rule_SubstRec \<le> (cc rule_SubstRec)\<^sup>*\<^sup>* OO (cc rule_SubstRec)\<^sup>*\<^sup>*\<inverse>\<inverse>"
 proof(rule joinI; elim rule_SubstRec.cases; clarify; goal_cases)
@@ -134,99 +141,82 @@ proof(rule joinI; elim rule_SubstRec.cases; clarify; goal_cases)
 
     have helper: "\<And> P x y. x = y \<Longrightarrow> P\<^sup>*\<^sup>* x y" by simp
 
-    have inj: "substVC (Suc (Suc n)) (Var 0) (liftVC 2 0 vc1) \<noteq>
-              substVC (Suc (Suc n)) (Var 0) (liftVC 2 0 vc2)" sorry
+    have inj: "renumber (id(Suc (Suc n):= 0)) (\<up> (\<up> vc1)) \<noteq>
+              renumber (id(Suc (Suc n):= 0)) (\<up> (\<up> vc2))" sorry
 
     show ?thesis
       apply (rule relcomppI)
        apply (rule rtranclp_trans[OF r_into_rtranclp r_into_rtranclp])
-        apply (simp only: liftV_appVC substV_appVC)
         apply (subst vc1_sub)
         apply (rule cc_rootI)
         apply (rule rule_SubstRec[OF _ refl refl])
-        apply (rule `occursE (n+1) e2`)
+        apply (rule `occurs (n+1) e2`)
       apply (subst subVC_swap[OF False[symmetric]])
       apply (rule congruentE[OF congruent_cc, of _ _ _  "[CUnir e]" for e, simplified appEC_def, simplified])
       apply (rule congruentE[OF congruent_cc, of _ _ _  "[CVal vc]" for vc, simplified appEC_def, simplified])
       apply (rule congruentE[OF congruent_cc, of _ _ _  "[CDef]", simplified appEC_def, simplified])
        apply (rule congruentE[OF congruent_cc, of _ _ _  "[CSeql e]" for e, simplified appEC_def, simplified])
        apply (rule cc_rootI)
-       apply (simp only: liftV_appVC[symmetric] substV_appVC[symmetric]) 
        apply (subst vc1_sub)
-       apply (simp only: liftV_appVC substV_appVC) 
+       apply (simp only: renumber_appVC) 
        apply (rule rule_SubstRec[OF _ refl refl])
-      using  `occursE (n+1) e2` apply (simp add: occursE_liftE)
+      using  `occurs (n+1) e2` apply (simp add: occurs_renumber renumber_renumber liftedN_def bumpAt_def)
+      apply fastforce
       apply (rule conversepI)
        apply (rule rtranclp_trans[OF r_into_rtranclp rtranclp_trans[OF r_into_rtranclp helper]])
-        apply (simp only: liftV_appVC substV_appVC)
         apply (subst vc2_sub)
         apply (rule cc_rootI)
         apply (rule rule_SubstRec[OF _ refl refl])
-       apply (rule `occursE (n+1) e1`)
+       apply (rule `occurs (n+1) e1`)
       apply (subst subVC_swap[OF False])
       apply (rule congruentE[OF congruent_cc, of _ _ _  "[CUnir e]" for e, simplified appEC_def, simplified])
       apply (rule congruentE[OF congruent_cc, of _ _ _  "[CVal vc]" for vc, simplified appEC_def, simplified])
       apply (rule congruentE[OF congruent_cc, of _ _ _  "[CDef]", simplified appEC_def, simplified])
        apply (rule congruentE[OF congruent_cc, of _ _ _  "[CSeql e]" for e, simplified appEC_def, simplified])
        apply (rule cc_rootI)
-       apply (simp only: liftV_appVC[symmetric] substV_appVC[symmetric]) 
        apply (subst vc2_sub)
-       apply (simp only: liftV_appVC substV_appVC) 
+       apply (simp only: renumber_appVC) 
        apply (rule rule_SubstRec[OF _ refl refl])
-      using  `occursE (n+1) e1` apply (simp add: occursE_liftE)
+      using  `occurs (n+1) e1` apply (simp add: occurs_renumber renumber_renumber liftedN_def bumpAt_def)
+      apply fastforce
       (* Now we have to show that the result is the same *)
-      apply (simp add: subVC_swap[OF False])
+      apply (simp add: subVC_swap[OF False] renumber_renumber  liftedN_def)
       apply (rule arg_cong2[where f = "\<lambda> e1 e2. appVC (subVC vc2 vc1 e1) e2" for vc1 vc2])
-      apply (rule arg_cong2[where f = VLet])
-        apply (rule arg_cong2[where f = appVC])
-         apply simp
-      apply (rule arg_cong2[where f = VLet])
+       apply (rule arg_cong2[where f = VLet, OF _ refl])
+       apply (rule arg_cong2[where f = appVC, OF refl])
+       apply (rule arg_cong2[where f = VLet])
          apply (rule arg_cong2[where f = appVC])
           apply (subst subVC_eq[OF False[symmetric] "1"(3)[symmetric]])
-          apply (simp add: liftVC_substVC)
-          apply (subst substVC_substVC)
-           apply simp
-          apply (simp add: substVC_dead)
-          apply (simp add: liftE_substE)
-          apply (subst substE_substE)
-           apply simp
-         apply (simp add: substE_dead occursE_liftE)
-          apply (simp add: liftE_substE)
-          apply (subst substE_substE)
-           apply simp
-        apply (simp add: substE_dead occursE_liftE)
-       apply simp
-      apply (rule arg_cong2[where f = VLet])
-       apply (simp add: liftVC_subVC substVC_subVC subVC_swap[OF inj])
-      apply (rule arg_cong2[where f = "\<lambda> e1 e2. appVC (subVC vc2 vc1 e1) e2" for vc1 vc2])
-      apply (rule arg_cong2[where f = VLet])
-         apply (rule arg_cong2[where f = appVC])
-          apply (subst (2) subVC_eq[OF False "1"(3), symmetric])
-          apply (simp add: liftVC_subVC substVC_subVC)
-          apply (rule arg_cong3[where f = subVC])
-            apply (simp add: liftVC_substVC)
-            apply (subst substVC_substVC)
-             apply simp
-            apply (simp add: substVC_dead)
-           apply (simp add: liftVC_substVC)
-           apply (subst substVC_substVC)
-            apply simp
-           apply (simp add: substVC_dead)
-          apply (simp add: liftE_substE)
-          apply (subst substE_substE)
-           apply simp
-         apply (simp add: substE_dead occursE_liftE)
-          apply (simp add: liftE_substE)
-          apply (subst substE_substE)
-           apply simp
-         apply (simp add: substE_dead occursE_liftE)
-          apply (simp add: liftE_substE)
-          apply (subst substE_substE)
-           apply simp
-         apply (simp add: substE_dead occursE_liftE)
-       apply simp
-      apply simp
+          apply (rule arg_cong[where f = "\<lambda>g. renumber g e" for e], rule)
+          apply (fastforce simp add: bumpAt_def)
+        apply (rule arg_cong[where f = "\<lambda>g. renumber g e" for e], rule)
+        apply (case_tac x) apply (fastforce simp add: liftedN_def)
+        apply (fastforce simp add: bumpAt_def liftedN_def)
+        apply (rule arg_cong[where f = "\<lambda>g. renumber g e" for e], rule)
+        apply (case_tac x) apply (fastforce simp add: liftedN_def bumpAt_def)
+        apply (fastforce simp add: bumpAt_def liftedN_def)
+      apply (rule arg_cong2[where f = VLet, OF _ refl])
+       apply (simp add: renumber_subVC add: subVC_swap[OF inj, unfolded renumber_renumber])
+       apply (rule arg_cong2[where f = "\<lambda> e1 e2. appVC (subVC vc2 vc1 e1) e2" for vc1 vc2])
+       apply (rule arg_cong2[where f = VLet])
+        apply (rule arg_cong2[where f = appVC])
+         apply (subst (2) subVC_eq[OF False "1"(3), symmetric])
+         apply (simp add: renumber_subVC)
+         apply (rule arg_cong3[where f = subVC])
+           apply (fastforce simp add: bumpAt_def liftedN_def renumber_renumber intro!: arg_cong[where f = "\<lambda>g. renumber g e" for e])
+          apply (fastforce simp add: bumpAt_def liftedN_def renumber_renumber intro!: arg_cong[where f = "\<lambda>g. renumber g e" for e])
+         apply (fastforce simp add: bumpAt_def liftedN_def renumber_renumber intro!: arg_cong[where f = "\<lambda>g. renumber g e" for e])
+        apply (simp add: renumber_renumber)
+        apply (rule arg_cong[where f = "\<lambda>g. renumber g e" for e], rule)
+        apply (case_tac x) apply (fastforce simp add: liftedN_def)
+        apply (fastforce simp add: bumpAt_def liftedN_def)
+       apply (simp add: renumber_renumber)
+       apply (rule arg_cong[where f = "\<lambda>g. renumber g e" for e], rule)
+       apply (fastforce simp add: bumpAt_def liftedN_def)
+      apply (rule arg_cong[where f = "\<lambda>g. renumber g e" for e], rule)
+      apply (fastforce simp add: bumpAt_def liftedN_def)
       done
+
   qed
 qed
 
